language/move-prover/bytecode-to-boogie/test_mvir/verify-vector.prover.bpl
@@ -1,0 +1,11 @@
+function {:inline 1} vector_length(v : Value) : Value {
+    Integer(vlen(v))
+}
+
+function {:inline 1} vector_get(v : Value, i : Value) : Value {
+    vmap(v)[i#Integer(i)]
+}
+
+function {:inline 1} vector_update(v : Value, i : Value, e : Value) : Value {
+    update_vector(v, i#Integer(i), e)
+}
